I2MP/Examples/Identity.v
@@ -4,10 +4,10 @@ Require Import Transitional.
 Require Import Source.Examples.Identity.
 
 Definition fuel := 200%nat.
-Definition to_run := compile_and_run_from_source_ex identity fuel.
+Definition to_run_tr := compile_and_run_from_source_ex identity fuel.
 
 Set Warnings "-extraction-reserved-identifier".
-Extraction "/tmp/run_mp_compiled_identity.ml" to_run.
+Extraction "/tmp/run_tagged_compiled_identity.ml" to_run_tr.
 
 
 Require Import Merged Int32.
@@ -18,3 +18,8 @@ Definition to_run_mr := @I2MP.Examples.Helper.compile_and_run_and_show_from_sour
 *)
 Set Warnings "-extraction-reserved-identifier".
 Extraction "/tmp/run_merged_compiled_identity.ml" to_run_mr.
+
+Require Import I2MP.Examples.Helper.
+
+Definition to_run := compile_and_run_mp identity fuel.
+Extraction "/tmp/run_mp_compiled_identity.ml" to_run.
