MicroPolicies/Instance.v
@@ -46,9 +46,9 @@ Definition reg0 : {fmap reg mt -> ratom } :=
       ; (as_word 19, Atom (as_word 0) Other)].
 
 
-Definition load (m : {fmap mword mt -> matom }) nc : state :=
-  {| Symbolic.mem := m ;
+Definition load (start : {fmap mword mt -> matom } * nat) nc : state :=
+  {| Symbolic.mem := fst start ;
      Symbolic.regs := reg0 ;
-     Symbolic.pc := {| vala := word.as_word 0 ; taga := Level 0 |} ;
+     Symbolic.pc := {| vala := word.as_word (snd start) ; taga := Level 0 |} ;
      Symbolic.internal := tt ;
      Symbolic.comp_num := nc|}.
