run_extracted_examples.sh
@@ -6,8 +6,9 @@ EXTRACTION_DIR=/tmp
 SOURCE_PREFIX="run_source_"
 INTERMEDIATE_PREFIX="run_intermediate_compiled_"
 TARGET_PREFIX="run_target_compiled_"
-MP_PREFIX="run_mp_compiled_"
+TAGGED_PREFIX="run_tagged_compiled_"
 MERGED_PREFIX="run_merged_compiled_"
+MP_PREFIX="run_mp_compiled_"
 
 if (( $# == 1 )); then
     if [[ $1 = "--force-extraction" ]]; then
@@ -56,6 +57,18 @@ for example in $TARGET_PREFIX*.ml; do
     ocaml nums.cma big.cma $example
 done
 
+
+# run compiled examples at the "tagged" level
+echo "*** Examples compiled at the tagged level ***"
+for example in $TAGGED_PREFIX*.ml; do
+    [ -f "$example" ] || continue
+    # prepend big int import to each example
+    echo -e "open Big_int\n$(cat $example)" > $example
+    echo "Output of $example:"
+    ocaml nums.cma big.cma $example
+done
+
+
 # run compiled examples at the micro-policy level
 echo "*** Examples compiled at the micro-policy level ***"
 for example in $MP_PREFIX*.ml; do
@@ -76,6 +89,5 @@ for example in $MERGED_PREFIX*.ml; do
     echo "Output of $example:"
     ocaml nums.cma big.cma $example
 done
-
 
 popd
